\documentclass[a4paper, 12pt]{report}

\usepackage[a4paper]{geometry}
\geometry{a4paper,tmargin=1in,bmargin=1in}

\usepackage{amsmath}
\usepackage{amssymb}
\usepackage{amsfonts}

%Custom command to shorten mathbb for basic number sets
\newcommand{\bb}[1]{\mathbb{#1}}

%Custom command for defining problem{#}{theorem}proof:{text}blacksquare
\newcommand{\proof}[3]{
	\begin{enumerate}
		\item[\bf{Problem #1}] #2
		\begin{enumerate}
			\item[\bf{Proof:}]
			#3
		\end{enumerate}
	\end{enumerate}
	\begin{flushright}
		$\blacksquare$
	\end{flushright}
}

%Custom command for defining problem{#}{text}
\newcommand{\problem}[2]{
	\begin{enumerate}
		\item[\bf{Problem #1}] 
		#2
	\end{enumerate}
}

%Custom command for defining {item}{theorem}proof:{text}blacksquare
%does require \b{enum} ... \e{enum} or \problem
\newcommand{\subproof}[3]{
	\item[#1] #2
	\item[\bf{Proof:}]
	#3 
	\begin{flushright}
		$\blacksquare$
	\end{flushright}
}

\begin{document}

\title{Math 440 -- Real Analysis II \\ \vspace{7px} \large{Homework 1}}
\author{Amandeep Gill}
\maketitle

\problem{1}{
	Find the limit inferior and limit superior of each of the following sequences \{$s_n$\}. \\
	\subproof{(a)}{$s_n = 2 - \frac{1}{n}$}{
		\[\varlimsup\{s_n\}=\varliminf\{s_n\}=\lim\limits_{n\to\infty}{s_n}=2\]
	}
	\subproof{(b)}{$s_n = n \bmod{4}$}{
		For all $k \in \mathbb{N}$ the sequence $\{s_k, s_{k+1}, s_{k+2}, \ldots\}$ contains only the values $\{0, 1, 2, 3\}$. Thus $\forall{k}$, $0 \leqslant s_k \leqslant 3$, so
		\[\varlimsup \{s_n\} = 3 \]
		\[\text{And}\]
		\[\varliminf \{s_n\} = 0 \] 
	}
	\subproof{(c)}{
		$s_n = \left\{
				\begin{array}{ll}
					n & \text{if $n$ is even} \\
					\frac{1}{n} + \cos{\pi n} & \text{if $n$ is odd}
				\end{array}
			\right.
		$
	}{
		For all $n \in \bf{N}$, $\frac{1}{n} + \cos{\pi n} \leq n$, so the $\sup\{s_k, s_{k+1}, s_{k+2}, \ldots\}$ is dominated by the even terms of $s_n$. Therefore
		\[\varlimsup \{s_n\} = \lim\limits_{n \to \infty}{2n} = \infty\]
		By the same argument, the $\inf\{s_k, s_{k+1}, s_{k+2}, \ldots\}$ is dominated by the odd terms of $s_n$, which is split between two cases: $s_k = \frac{1}{k} + 1$ and $s_k = \frac{1}{k} - 1$. Thus
		\[\varliminf \{s_n\} = \lim\limits_{n\to\infty}{\frac{1}{4n+3}-1}= -1\]
	}
	\pagebreak
	\subproof{(d)}{$s_n = f(n)$, where $f \colon \mathbb{N} \to \mathbb{Q} \cap (0,1)$ is a bijection}{
		Let $\epsilon > 0$ and $\overline{S} = \{s_n \colon 1 - s_n < \epsilon\}$ \\
		By Math340 results we know that there exists an infinite number of rationals between any two distinct reals (in this case 1 and $1 - \epsilon$). Therefore $\overline{S}$ is a countably infinite set, and $\overline{S} \setminus \{s_1, s_2, \ldots, s_{k-1}\}$ yields a similarly infinite set. From this,
		\[\varlimsup \{s_n\} = \sup{\overline{S}} = 1\] 
		
		Similarly, with $\underline{S} = \{s_n \colon s_n < \epsilon\}$ we have 
		\[\varliminf \{s_n\} = \inf{\underline{S}} = 0\]
	}
}

\proof{2}{
	Give an example of a sequence $\{s_n\}$ and a real number $s$ such that $s_n < s$ for all $n$, but $\varlimsup s_n \geqslant s$
}{
	Let $s_n = 1-\frac{1}{n}$ and $s = 1$, then $\forall n, s_n < s$ and $\varlimsup s_n = s$
}

\proof{3}{
	Let \{$a_n$\} and \{$b_n$\} be bounded sequences of nonnegative real numbers.
}{
	$\varlimsup(a_n b_n) \leqslant (\varlimsup a_n)(\varlimsup b_n)$
}{
	Since $a_n, b_n$ are bounded and nonnegative, let $A,B \in \mathbb{R}^+ \cup  \{0\}$ such that $\varlimsup \{a_n\} = A$ and $\varlimsup \{b_n\} = B$ \\
	By definition, $\forall n, a_n \leqslant A$ and $b_n \leqslant B$, so $a_n b_n \leqslant AB$ \\
	$AB$ is thus an upper bound on the sequence $\{a_n b_n\}$ \\ 
	Therefore $\varlimsup \{a_n b_n\} \leqslant AB$	
}

\proof{4}{
	The series $\sum\limits_{k=1}^{\infty} \frac{1}{\sqrt{k}}$ diverges
}{
	Let $s_n = \sum\limits_{k=1}^{n} \frac{1}{\sqrt{k}}$ \\
	Then $s_n = 1 + \frac{1}{\sqrt{2}} + \cdots + \frac{1}{\sqrt{n}}$ \\
	Since $\frac{1}{\sqrt{k}}$ is monotone decreasing, we have
	\[
		s_n \geqslant 
		\frac{1}{\sqrt{n}} + \frac{1}{\sqrt{n}} + \cdots \frac{1}{\sqrt{n}}
		= \frac{n}{\sqrt{n}} = \sqrt{n}
	\]
	So for all $n \geqslant 1$, the partial sum $s_n \geqslant \sqrt{n}$ \\
	Therefore, $\varlimsup\{s_n\} \geqslant \varlimsup\{\sqrt{n}\} = \infty$ 
}
\pagebreak
\proof{5}{
	Let $\{a_n\}_{n\in\mathbb{N}}$ be a sequence of real values. \\
	The series $\sum\limits_{n=1}^{\infty}(a_n - a_{n+1})$ converges if and only if $\{a_n\}$ converges.
}{
	Let $s_n = \sum\limits_{k=1}^{n}(a_k - a_{k+1})$ \\
	The partial sums $s_n$ are telescoping sums, so $\forall n, s_n = a_1 - a_{n+1}$ \\
	Therefore, $\lim\limits_{n \to \infty} s_n = \lim\limits_{n \to \infty} a_1 - a_n = a_1 - \lim\limits_{n \to \infty} a_n$ \\
	Since $\lim\limits_{n \to \infty} a_n$ exists if and only if $\exists A \in \mathbb{R}$ such that $\{a_n\} \to A$ \\
	$\{s_n\}$ converges to $a_1 - A$ if and only if $\{a_n\}_{n\in\mathbb{N}}$ converges to $A$
}
\proof{6}{
	$\sum\limits_{k=1}^{\infty}\frac{2}{k(k+1)} = 2$
}{
	By partial fraction decomposition, $\frac{2}{2(k+1)} = \frac{2}{k} - \frac{2}{k+1}$ \\
	Let $a_k = \frac{2}{k}$, then $a_1 = 2$ and $\lim\limits_{k \to \infty} a_k = 0$ \\
	Therefore by previous work, \\
	$\sum\limits_{k=1}^{\infty}(a_k - a_{k+1}) = a_1 - \lim\limits_{n \to \infty}a_n = 2 - 0 = 2$
}
\proof{7}{
	$\sum\limits_{k=1}^{\infty}(\sqrt{k+1} - \sqrt{k})$ diverges
}{
	Let $a_k = - \sqrt{k}$ \\
	$\sum\limits_{k=1}^{\infty}(\sqrt{k+1} - \sqrt{k}) = \sum\limits_{k=1}^{\infty}(a_k - a_{k+1})$ \\
	Since $\{a_k\}$ diverges, the series diverges by previous results.
}

\end{document}
